theories/lang/cpp/logic/pred.v
@@ -203,6 +203,8 @@ Module Type CPP_LOGIC
       #[global] Declare Instance reference_to_knowledge : Knowledge2 reference_to.
       #[global] Declare Instance reference_to_timeless : Timeless2 reference_to.
 
+      (* NOTE: this is almost derivable from [reference_to_intro] and
+         [reference_to_elim] except for the issue with non-standard types. *)
       Axiom reference_to_erase : forall ty p,
           reference_to ty p -|- reference_to (erase_qualifiers ty) p.
 
@@ -250,8 +252,37 @@ Module Type CPP_LOGIC
       Timeless (provides_storage storage_ptr obj_ptr ty).
     #[global] Existing Instances provides_storage_persistent provides_storage_affine provides_storage_timeless.
 
-    (**
-    Typed points-to predicate. Fact [tptsto t q p v] asserts the following things:
+    (** Heap types.
+    The [t : type] in this definition is a "heap type", it is *completely*
+    unqualified.
+    - Top-level <<const>> qualifiers, e.g. the <<const>> in <<int * const>>, are
+      tracked in the <<const>> bit of [cQp.t].
+    - Memory cells that are marked <<volatile>> are currently not supported and
+      will use a different ownership discipline, i.e. not using [tptsto] at all.
+    - Nested qualifiers are normalized in these definitions due to sub-typing
+      constraints.
+    - Top-level references are uniformly represented using [Tref], i.e. [Trv_ref]
+      does not occur at the toplevel.
+
+    Some examples of the above include:
+    - <<const int x = 1>>           -- [tptsto Tint (cQp.m 1) _ 1]
+    - <<const int* x = nullptr>>    -- [tptsto (Tptr Tint) (cQp.m 1) _ nullptr]
+    - <<int* const x = nullptr>>    -- [tptsto (Tptr Tint) (cQp.c 1) _ nullptr]
+    - <<volatile int x = 0>>        -- not represted using [tptsto]
+    - <<volatile int* p = nullptr>> -- [tptsto (Tptr Tint) (cQp.m 1) _ nullptr]
+    - <<int&& r = ..>>              -- [tptsto (Tref Tint) (cQp.m 1) _ _]
+     *)
+    Parameter is_heap_type : type -> bool.
+    Axiom is_heap_type_eq :
+      is_heap_type = fun t =>
+                       bool_decide (t = erase_qualifiers t)
+                    && (is_value_type t || match t with
+                                          | Tref _ => true
+                                          | _ => false
+                                          end).
+
+    (** *** Typed points-to predicate.
+    Fact [tptsto t q p v] asserts the following things:
     1. Pointer [p] points to value [v].
     2. We have fractional ownership [q] (in the separation logic sense).
     3. Pointer [p] points to a memory location with C++ type [t].
@@ -259,10 +290,21 @@ Module Type CPP_LOGIC
     1. Value [v] need not be initialized.
     2. Hence, [v] might not satisfy [has_type_prop t v].
 
+    [tptsto] is only used to represent memory cells that contain
+    values representable as a single [val]. This includes:
+    - value types (see [is_value_type]), and
+    - reference types. Note that all glvalues, i.e. x-values ([Trv_ref])
+      and l-values ([Tref]), are represented using [Tref].
+    These requirements justify the axiom [tptsto_valid_type].
+
     We use this predicate both for pointers to actual memory and for pointers to
     C++ locations that are not stored in memory (as an optimization).
     *)
     Parameter tptsto : forall {σ:genv} (t : type) (q : cQp.t) (a : ptr) (v : val), mpred.
+
+    #[global] Declare Instance tptsto_valid_type
+      : forall {σ:genv} (t : type) (q : cQp.t) (a : ptr) (v : val),
+        Observe [| is_heap_type t |] (tptsto t q a v).
 
     Axiom tptsto_nonnull : forall {σ} ty q a,
       @tptsto σ ty q nullptr a |-- False.
